Flapjack/Tests.lean
@@ -577,6 +577,15 @@ example :
     loopCompileExps, loopNestedSeq, loopTempNames, wordFindVar, lookupInfo,
     lookupNatInfo]
 
+example [NeZero width] :
+    pipelineRiscVFunctions
+        (width := width)
+        [(0, [], ((.seq (.assign 1 (.op .add [.var 2, .var 3]))
+          (.return 0 [1])) : WordProg (RiscV.Word width)))] =
+      [(0, [], some ([.add 1 2 3], [1]))] := by
+  simp [pipelineRiscVFunctions, RiscV.wordFunctionToRiscV,
+    RiscV.wordExpToInstruction, RiscV.registerOfNat]
+
 example :
     let result := compileFlapjack (α := Nat) .rv64i 1 id
       [.decl .one "g" (.const 7), .function
